theories/Misc/Pure.v
@@ -1,0 +1,300 @@
+From CTree Require Import
+     Eq Eq.Epsilon.
+
+Variant pureb {E C X} (rec : ctree E C X -> Prop) (t : ctree E C X) : Prop :=
+  | pureb_ret   (v : X) (EQ : t ≅ Ret v) : pureb rec t
+  | pureb_delay {Y} (c: C Y) k (EQ : t ≅ BrD c k) (REC: forall v, rec (k v)) : pureb rec t.
+
+Program Definition fpure {E C R} : mon (ctree E C R -> Prop) := {|body := pureb|}.
+Next Obligation.
+  inversion_clear H0; [eleft | eright]; eauto.
+Qed.
+
+Section pure.
+
+  Context {E C : Type -> Type} {X : Type}.
+
+  Class pure (t : ctree E C X) := pure_ : gfp (@fpure E C X) t.
+
+  #[global] Instance pure_equ : Proper (@equ E C X X eq ==> flip impl) pure.
+  Proof.
+    cbn. intros. step in H0. inversion H0.
+    - step. eleft. now rewrite H, EQ.
+    - step. eright. now rewrite H, EQ. apply REC.
+  Qed.
+
+  #[global] Instance pure_ret r : pure (Ret r).
+  Proof.
+    step. now eleft.
+  Qed.
+
+  #[global] Instance pure_br {T} (c : C T) k :
+    (forall x, pure (k x)) ->
+    pure (BrD c k).
+  Proof.
+    intros. step. now eright.
+  Qed.
+
+  #[global] Instance pure_guard `{B1 -< C} t :
+    pure t ->
+    pure (Guard t).
+  Proof.
+    intros. unfold Guard. step. now eright.
+  Qed.
+
+  #[global] Instance pure_stuck `{B0 -< C} :
+    pure stuckD.
+  Proof.
+    unfold stuckD. step. now eright.
+  Qed.
+
+  Lemma pure_brD_inv : forall {X} (c : C X) k x,
+    pure (BrD c k) ->
+    pure (k x).
+  Proof.
+    intros. step in H. inv H; inv_equ.
+    rewrite EQ0. apply REC.
+  Qed.
+
+  Lemma pure_productive : forall (t : ctree E C X),
+    pure t -> productive t -> exists r, t ≅ Ret r.
+  Proof.
+    intros. step in H. inv H; eauto.
+    rewrite EQ in H0. inv H0; inv_equ.
+  Qed.
+
+  Lemma pure_epsilon :
+    forall t t', pure t -> epsilon t t' -> pure t'.
+  Proof.
+    intros. rewrite ctree_eta in H. rewrite ctree_eta. red in H0. genobs t ot. genobs t' ot'.
+    clear t t' Heqot Heqot'. induction H0.
+    - now subs.
+    - apply IHepsilon_. rewrite <- ctree_eta. eapply pure_brD_inv. apply H.
+  Qed.
+
+  Lemma trans_pure_is_val `{B0 -< C} (t t' : ctree E C X) l :
+    pure t ->
+    trans l t t' ->
+    is_val l.
+  Proof.
+    intros. do 3 red in H1. genobs t ot. genobs t' ot'.
+    assert (t ≅ go ot). { now rewrite Heqot, <- ctree_eta. } clear Heqot.
+    revert t H0 H2. induction H1; intros; subst.
+    - apply IHtrans_ with (t := k x); auto. 2: apply ctree_eta.
+      rewrite H2 in H0. step in H0. inversion H0; inv_equ.
+      rewrite EQ0. apply REC.
+    - rewrite H2 in H1. step in H1. inversion H1; inv_equ.
+    - rewrite H2 in H1. step in H1. inversion H1; inv_equ.
+    - constructor.
+  Qed.
+
+  Lemma trans_bind_pure {Y} `{B0 -< C} (t : ctree E C X) k (u : ctree E C Y) l :
+    pure t ->
+    trans l (CTree.bind t k) u ->
+    exists v, trans (val v) t stuckD /\ trans l (k v) u.
+  Proof.
+    intros. apply trans_bind_inv in H1 as [(? & ? & ? & ?) |].
+    - now apply trans_pure_is_val in H2.
+    - apply H1.
+  Qed.
+
+End pure.
+
+#[global] Instance pure_map {E B X Y} : forall (t : ctree E B X) (f : X -> Y),
+  pure t ->
+  pure (CTree.map f t).
+Proof.
+  red. coinduction R CH. intros.
+  step in H. destruct H.
+  - eleft. rewrite EQ. rewrite map_ret. reflexivity.
+  - eright.
+    + rewrite EQ. unfold CTree.map. rewrite bind_br. reflexivity.
+    + intros. apply CH. apply REC.
+Qed.
+
+Section pure_finite.
+
+  Context {E C : Type -> Type} {X : Type}.
+
+  Inductive pure_finite_ : ctree E C X -> Prop :=
+    | puref_ret (v : X) t (EQ: t ≅ Ret v) : pure_finite_ t
+    | puref_delay {Y} (c: C Y) (k : Y -> ctree E C X) t (EQ: t ≅ BrD c k) (REC: forall v, pure_finite_ (k v)) : pure_finite_ t.
+
+  Class pure_finite (t : ctree E C X) : Prop :=
+    pure_finite__ : pure_finite_ t.
+
+  #[global] Instance pure_finite_equ :
+    Proper (equ eq ==> flip impl) pure_finite.
+  Proof.
+    cbn. intros. revert x H. induction H0; intros.
+    - eleft. now subs.
+    - eright. now subs.
+      intro. now eapply H.
+  Qed.
+
+  #[global] Instance pure_finite_ret r : pure_finite (Ret r).
+  Proof.
+    now eleft.
+  Qed.
+
+  #[global] Instance pure_finite_br {T} (c : C T) k :
+    (forall x, pure_finite (k x)) ->
+    pure_finite (BrD c k).
+  Proof.
+    now eright.
+  Qed.
+
+  #[global] Instance pure_finite_guard `{B1 -< C} t :
+    pure_finite t ->
+    pure_finite (Guard t).
+  Proof.
+    unfold Guard. now eright.
+  Qed.
+
+  #[global] Instance pure_finite_stuck `{B0 -< C} :
+    pure_finite stuckD.
+  Proof.
+    unfold stuckD. now eright.
+  Qed.
+
+End pure_finite.
+
+Lemma pure_finite_bind_R {E C X Y} :
+  forall R t (k : X -> ctree E C Y),
+  t (≅R) t ->
+  pure_finite t ->
+  (forall x, R x x -> pure_finite (k x)) ->
+  pure_finite (CTree.bind t k).
+Proof.
+  intros. induction H0.
+  - subs. inv_equ. rewrite bind_ret_l; auto.
+  - subs. inv_equ. rewrite bind_br. apply pure_finite_br. auto.
+Qed.
+
+#[global] Instance pure_finite_bind {E C X Y} :
+  forall t (k : X -> ctree E C Y),
+  pure_finite t ->
+  (forall x, pure_finite (k x)) ->
+  pure_finite (CTree.bind t k).
+Proof.
+  intros. apply (pure_finite_bind_R eq); auto.
+Qed.
+
+#[global] Instance pure_pure_finite {E C X} :
+  forall (t : ctree E C X),
+  pure_finite t ->
+  pure t.
+Proof.
+  intros. induction H; subs; step.
+  - now eleft.
+  - now eright.
+Qed.
+
+Lemma is_stuck_pure : forall {E B X Y} `{B0 -< B} t (k : X -> ctree E B Y),
+  pure t ->
+  (forall x, is_stuck (k x)) ->
+  is_stuck (CTree.bind t k).
+Proof.
+  red. intros. intro.
+  apply trans_bind_inv in H2 as [].
+  - destruct H2 as (? & ? & ? & ?). subs.
+    apply H2. eapply trans_pure_is_val; eauto.
+  - destruct H2 as (? & ? & ?). now apply H1 in H3.
+Qed.
+
+(*|
+A computation [is_simple] all its transitions are either:
+- directly returning
+- or reducing in one step to something of the shape [Guard* (Ret r)]
+|*)
+Class is_simple {E C X} (t : ctree E (B01 +' C) X) :=
+  is_simple' : (forall l t', trans l t t' -> is_val l) \/
+  (forall l t', trans l t t' -> exists r, epsilon_det t' (Ret r)).
+
+
+Section is_simple_theory.
+
+  Context {E C : Type -> Type} {X : Type}.
+
+  #[global] Instance is_simple_equ :
+    Proper (equ eq ==> iff) (@is_simple E C X).
+  Proof.
+    cbn. intros. unfold is_simple. setoid_rewrite H. reflexivity.
+  Qed.
+
+  #[global] Instance is_simple_ret : forall r, is_simple (Ret r : ctree E (B01 +' C) X).
+  Proof.
+    cbn. red. intros. left. intros. inv_trans. subst. constructor.
+  Qed.
+
+  #[global] Instance is_simple_guard_ret : forall r,
+      is_simple (Guard (Ret r) : ctree E (B01 +' C) X).
+  Proof.
+    cbn. red. intros. left. intros. inv_trans. subst. constructor.
+  Qed.
+
+  #[global] Instance is_simple_br : forall (c: (B01 +' C) X),
+      is_simple (branchD c : ctree E (B01 +' C) X).
+  Proof.
+    cbn. red. intros.
+    left. intros. apply trans_brD_inv in H as []. inv_trans. subst. constructor.
+  Qed.
+
+  #[global] Instance is_simple_map :
+    forall {Y} (t : ctree E (B01 +' C) X) (f : X -> Y),
+    is_simple t -> is_simple (CTree.map f t).
+  Proof.
+    intros. destruct H.
+    - left. intros.
+      unfold CTree.map in H0. apply trans_bind_inv in H0 as ?.
+      destruct H1 as [(? & ? & ? & ?) | (? & ? & ?)].
+      + now apply H in H2.
+      + apply trans_ret_inv in H2 as []. now subst.
+    - right. intros.
+      apply trans_bind_inv in H0 as ?.
+      destruct H1 as [(? & ? & ? & ?) | (? & ? & ?)].
+      + apply H in H2 as []. exists (f x0). subs.
+        eapply Epsilon.epsilon_det_bind_ret_l. apply H2. reflexivity.
+      + apply H in H1 as []. inv H1; inv_equ.
+  Qed.
+
+  #[global] Instance is_simple_liftState {St} :
+    forall (t : ctree E (B01 +' C) X) (s : St),
+    is_simple t -> is_simple (Monads.liftState t s).
+  Proof.
+    intros. cbn. typeclasses eauto.
+  Qed.
+
+  #[global] Instance is_simple_trigger :
+    forall (e : E X),
+    is_simple (CTree.trigger e : ctree E (B01 +' C) X).
+  Proof.
+    right. intros.
+    unfold CTree.trigger in H. inv_trans. subst.
+    exists x. now left.
+  Qed.
+
+  Lemma is_simple_brD : forall {Y} (c: (B01 +' C) X) (k : X -> ctree E (B01 +' C) Y) x,
+      is_simple (BrD c k) -> is_simple (k x).
+  Proof.
+    intros. destruct H.
+    - left. intros. eapply H. etrans.
+    - right. intros. eapply H. etrans.
+  Qed.
+
+  #[global] Instance is_simple_pure :
+    forall (t : ctree E (B01 +' C) X),
+    pure t -> is_simple t.
+  Proof.
+    left. intros. eapply trans_pure_is_val; eassumption.
+  Qed.
+
+End is_simple_theory.
+
+(*|
+A computation is [vsimple] if it is syntactically:
+- a [Ret]
+- or a [trigger]
+|*)
+Definition vsimple {E C X} (t : ctree E (B01 +' C) X) :=
+  (exists x, t ≅ Ret x) \/ exists f, t ≅ CTree.trigger f.
